	\documentclass[10pt,a4paper]{report}
\usepackage[utf8]{inputenc}
\usepackage{amsmath}
\usepackage{amsfonts}
\usepackage{amssymb}
\usepackage{amsthm}
\usepackage{hyperref}

\usepackage{multicol}
\usepackage{fancyhdr}
\usepackage{enumitem}
\usepackage{tikz}
\usepackage{tikz-cd}
\usetikzlibrary{calc}
\usetikzlibrary{shapes.geometric}
\usepackage[margin=0.5in]{geometry}
\usepackage{xcolor}
\DeclareMathOperator{\RANGE}{range}
\DeclareMathOperator{\NULL}{null}

\hypersetup{
    colorlinks=true,
    linkcolor=blue,
    filecolor=magenta,      
    urlcolor=cyan,
    pdftitle={Tensors},
    pdfpagemode=FullScreen,
    }

%\urlstyle{same}

\newcommand{\CLASSNAME}{Functional Analysis}
\newcommand{\STUDENTNAME}{Paul Carmody}
\newcommand{\ASSIGNMENT}{Assignment \#5}
\newcommand{\DUEDATE}{April 18, 2024}
\newcommand{\SEMESTER}{Spring 2024}
\newcommand{\SCHEDULE}{T/Th 9:30 -- 10:45}
\newcommand{\ROOM}{Remote}

\pagestyle{fancy}
\fancyhf{}
\chead{ \fancyplain{}{\CLASSNAME} }
%\chead{ \fancyplain{}{\STUDENTNAME} }
\rhead{\thepage}
\input{../MyMacros}

\newcommand{\RED}[1]{\textcolor{red}{#1}}
\newcommand{\BLUE}[1]{\textcolor{blue}{#1}}
\newcommand{\GREEN}[1]{\textcolor{black!30!green}{#1}}
\newcommand{\ORANGE}[1]{\textcolor{orange}{#1}}
\newcommand{\F}{\textbf{F}}
\newcommand{\NLL}{\mathcal{N}}

\title{Advanced Linear Algebra}
\author{The Unforgetable Someone}
\date{Summer 2023}

\newcommand{\NORM}[1]{\,\left \Vert #1 \right \Vert}
\begin{document}

\begin{center}
	\Large{\CLASSNAME -- \SEMESTER} \\
\end{center}
\begin{center}
	\STUDENTNAME \\
	\ASSIGNMENT -- \DUEDATE\\
\end{center} 

p. 200 \#2,3,4,5,6,10. 
\begin{enumerate}
	\setcounter{enumi}{1}
	\item Let $H$ be a Hilbert space and $T: H \to H$ a bijective bounded linear operator whose inverse is bounded.  Show that $(T^*)^{-1}$ exists and 
	\begin{align*}
		(T^*)^{-1}=(T^{-1})^*
	\end{align*}
	
	\begin{align*}
		(TT^*)^{-1} &= (T^*)^{-1}T^{-1} \\
		(TT^*)^{-1}T &= (T^*)^{-1}\\
		\therefore (T^*)^{-1} &\text{ exists}\\
		\\
		\ABRACKET{Tx, y} &= \ABRACKET{x, T^*y}\\
		\ABRACKET{T^{-1}Tx, y} &= \ABRACKET{T^{-1}x, T^*y}\\
		\ABRACKET{x,y} &= \ABRACKET{T^{-1}x, T^*y}\\
		\ABRACKET{x, (T^*)^{-1}y} &= \ABRACKET{T^{-1}x, (T^*)^{-1}T^*y}\\
		&= \ABRACKET{T^{-1}x, y} \\
		&= \ABRACKET{x, (T^{-1})^*y} \\
		(T^*)^{-1}&=(T^{-1})^*
	\end{align*}
	
	\item If $(T_n)$ is a sequence of bounded linear operators on a Hilbert space and $T_n \to T$, show that $T_n^*\to T^*$.
	
	\begin{align*}
		\NORM{T_n -T}^2 &\ge \NORM{T_n}^2 - \NORM{T}^2 = \NORM{T_n^*}^2 - \NORM{T^*}^2 \ge \NORM{T_n^*-T^*}^2\\
		\text{similarly, }  \NORM{T_n^*-T^*}^2 &\ge  \NORM{T_n^*}^2 - \NORM{T^*}^2 = \NORM{T_n}^2 - \NORM{T}^2 \ge \NORM{T_n -T}^2 \\
		\text{hence } \NORM{T_n -T}^2 &= \NORM{T_n^*-T^*}^2
	\end{align*}	We know that given any $N>0$ then for all $n > N$ when $\NORM{T_n -T} < \epsilon$ implies that $\NORM{T_n^*-T^*}<\epsilon$.  Therefore, $T_n^* \to T^*$.
	
	\item Let $H_1$ and $H_2$ be Hilbert spaces and $T: H_1 \to H_2$ a bounded linear operator.  If $M_1\subset H_1$ and $M_2 \subset H_2$ are such that $T(M_1) \subset M_2$, show that $M_1^\perp \subset T^*(M_2^\perp)$.
	
	 Let $x \in M_1$ and $z \in M_2^\perp$ and $x \not \in \mathcal{N}(T)$.Then, $\ABRACKET{Tx, z}=0$ implies $\ABRACKET{x, T^*z}=0$ and either $T^*z \in \mathcal{N}(T^*)$ or $T^*z \perp x$.  $x$ is arbitrary, therefore $T^*z \perp \SPAN(M_1)$ or $T^*z \in M_1^\perp$.  Thus, $T^*z \in \mathcal{N}(T^*) \cup M_1^\perp$.  $z$ is arbitrary so $T^*(M_2^\perp) = \mathcal{N}(T^*) \cup M_1^\perp$, hence, $M_1^\perp \subset T^*(M_2^\perp)$.
	
	\item Let $M_1$ and $M_2$ in Prob. 4 be closed subspaces.   Show that $T(M_1)\subset M_2$ if and only if $M_1^\perp \supset T^*(M_2^\perp)$.
	
	$(\Rightarrow)$ Assuming that $T(M_1) \subset M_2$.  We can see that $H_1 = M_1 \oplus M_1^\perp$.  Then, let $x \in H_1, x= a+b$ for some $a \in M_1$ and $b \in M_1^\perp$ and $z \in M_2^\perp$ such that $z \ne 0$.  Then, 
	\begin{align*}
		\ABRACKET{Tx, z} &= \ABRACKET{Ta,z}+\ABRACKET{Tb,z} \\
		&= \ABRACKET{Tb,z} \\
		&= \ABRACKET{b, T^*z} \\
		z \ne 0 &\implies T^*z \in M_1^\perp
	\end{align*}$z$ is arbitrary, thus $T^*(M_2^\perp) \subset M_1^\perp$.
	
	$(\Leftarrow)$ Assuming that $M^\perp \supset T^*(M_2^\perp)$.  We can see that $H_2 = M_2 \oplus M_2^\perp$.  Then, let $z \in H_2, z= c+d$ for some $c\in M_2$ and $d\in M_2^\perp$ and $x \in M_1$ and $x\ne 0$.  Then,
	\begin{align*}
		\ABRACKET{x, T^*z} &= \ABRACKET{x, T^*c}+\ABRACKET{x, T^*d} \\
		&= \ABRACKET{x,T^*c} \\
		&= \ABRACKET{Tx, c} \\
		x \ne 0 & \implies Tx \in M_2
	\end{align*}$x$ is arbitrary, thus $T(M_1) \subset M_2$
	
	\item If $M_1=\mathcal{N}(T)=\{x\,|\,Tx=0\}$ in Prob. 4, show that 
	\begin{enumerate}
		\item $T^*(H_2) \subset M_1^\perp$
		
		$\mathcal{N}(T)$ is a closed vector space and by Prob 5 we can see that if $M_2=\{0\}$ then $M_2^\perp = H_2$.  Thus, $T^*(M_2^\perp)=T^*(H_2)\subset M_1^\perp$.
		
		\item $[T(H_1)]^\perp \subset \mathcal{N}(T^*)$
		
		Let $x \in H_1 \backslash \NLL(T)$ and $z \in \NLL(T^*)$ then $0=\ABRACKET{x, T^*z}=\ABRACKET{Tx, z}$ implies that $Tx \in \NLL(T^*)^\perp$.\\
		Since $H_1=\NLL(T)\oplus \NLL(T)^\perp$ given any $x \in \NLL(T)$ then $Tx = 0 \in \NLL(T^*)$ or $x \in \NLL(T)^\perp$ then $Tx\in \NLL(T^*)^\perp$, then $[T(H_1)]^\perp \subset \NLL(T^*)$.
		
		\item $M_1=[T^*(H_2)]^\perp$
		
		Let $z \in H_2\backslash \NLL(T^*)$ and $x \in \NLL(T)$ then $0 = \ABRACKET{Tx, z}= \ABRACKET{x, T^*z}$ implies that $T^*z \in \NLL(T)^\perp$.\\
		Since $H_2 = \NLL(T^*)\oplus \NLL(T^*)^\perp$ given any $z\in \NLL(T^*)$ then $T^*z = 0 \in \NLL(T)$ or $z \in \NLL(T^*)^\perp$ then $T^*z \in \NLL(T)^\perp$,\\
		then $[T^*(H_2)]^\perp = \NLL(T)$.
	\end{enumerate}
	\setcounter{enumi}{9}
	\item \textbf{(Right shift operator)} Let $(e_n)$ be a total orthonormal sequence in a separable Hilbert space $H$ and define the \textit{right shift operator} to be the linear operator $T: H \to H$ such that $Te_n=e_{n+1}$ for $n=1,2,\cdots$.  Explain the name.  Find the range, null space, norm and Hilbert-adjoint operator of $T$.\\
	
	The \textit{right shift operator} gets its name by shifting the element back one position.\\
	The range of $\mathcal{R}(T)$ is the set of total orthornormal sequences.\\
	The null space is the first element if $e_1 = 1, 0, 0, 0, \dots $ for clearly $Te_1 = (0)$.  \\
	The norm $\NORM{T} = \SUP{x \in H, \NORM{x}=1} Tx = 1$\\
	The adjoint, $T^*$, note that 
	\begin{align*}
		\ABRACKET{Te_i, e_j} &= \ABRACKET{e_{i+1}, e_j} = \BINDEF{ 1 & j = i+1 }{0 & \text{otherwise}} \\
		\text{ then }&\\
		\ABRACKET{e_i, T^*e_j} &= \ABRACKET{Te_i, e_j} \\
		& \implies T^*e_j = e_{j-1}
	\end{align*}

\end{enumerate}

\newpage
p. 207 \#4, 5

\begin{enumerate}
	\setcounter{enumi}{3}
	\item Show that for any bounded linear operator $T$ on $H$, the operators 
	\begin{align*}
		T_1=\frac{1}{2}(T+T^*) \text{  and  } T_2=\frac{1}{2i}(T-T^*)
	\end{align*}are self-adjoint.  Show that 
	\begin{align*}
		T=T_1+iT_2 \text{ and }  T^*=T_1-iT_2.
	\end{align*}Show uniqueness, that is, $T_1+iT_2=S_1+iS_2$ implies $S_1=T_1$ and $S_2=T_2$; here, $S_1$ and $S_2$ are self-adjoint by assumption.

\begin{multicols}{2}	
	\begin{align*}
		T_1&=\frac{1}{2}(T+T^*) \\
		\ABRACKET{T_1x, y} &= \ABRACKET{\PAREN{\frac{1}{2}(T+T^*)}x, y} \\
		&= \frac{1}{2}\ABRACKET{Tx+T^*x, y} \\
		&= \frac{1}{2}\PAREN{\ABRACKET{Tx, y} +\ABRACKET{T^*x, y} }\\
		&= \frac{1}{2}\PAREN{\ABRACKET{x, T^*y} + \ABRACKET{x, Ty}} \\
		&= \frac{1}{2}\ABRACKET{x, T^*y +  Ty} \\
		&= \ABRACKET{x, \frac{1}{2}\PAREN{T^*y +  Ty}} \\
		&= \ABRACKET{x, T_1y}
	\end{align*}
	
	\begin{align*}
		T_2&=\frac{1}{2i}(T-T^*) \\
		\ABRACKET{x, T_2y} &= \ABRACKET{x, \frac{1}{2i}\PAREN{T-T^*} y} \\
		&= \frac{-1}{2}\ABRACKET{x, Ty-T^*y} \\
		&= \frac{-1}{2}\PAREN{\ABRACKET{x, Ty} -\ABRACKET{x, T^*y} }\\
		&= \frac{-1}{2}\PAREN{\ABRACKET{T^*x, y} - \ABRACKET{Tx, y}} \\
		&= \frac{-1}{2}\ABRACKET{T^*x -  Tx, y} \\
		&= \ABRACKET{\frac{-1}{2}\PAREN{T^*x -  Tx}, y} \\
		&= \ABRACKET{T_2x, y}
	\end{align*}	
\end{multicols}
\begin{multicols}{2}
	\begin{align*}
		T_1+iT_2 &= \frac{1}{2}(T+T^*) + \frac{1}{2i}(T-T^*) \\
		&= \frac{1}{2}T+\frac{1}{2}T^* + \frac{1}{2}T-\frac{1}{2}T^* \\
		&= T
	\end{align*}
	\begin{align*}
\\		T_1-iT_2 &= \frac{1}{2}(T+T^*) - \frac{1}{2i}(T-T^*) \\
		&= \frac{1}{2}T+\frac{1}{2}T^* - \frac{1}{2}T+\frac{1}{2}T^* \\
		&= T^*
	\end{align*}
\end{multicols}

	\item On $\C^2$ (cf. 3.1-4) let the operator $T: \C^2\to \C^2$ be defined by $Tx=(\xi_1+i\xi_2, \xi_1-i\xi_2),$ where $x=(\xi_1,\xi_2)$.  Find $T^*$.  Show that we have $T^*T=TT^*=2I$.  Find $T_1$ and $T_2$ as defined in prob. 4.

	\begin{align*}
		T(a+bi) &= a+ib+i(a-ib) = a+b+i(a+b) = (a+b)(1+i) \\
		\ABRACKET{T(a+bi), c+di} &= \ABRACKET{(a+b)(1+i), c+di}= (a+b)\ABRACKET{1+i,c+di} = (a+b)(c+d)\\
		(a+b)(c+d) &= \ABRACKET{a+bi, 1+i}(c+d) = \ABRACKET{a+bi, (c+d)(1+i)} \\
		T^*(c+di) &= (c+d)(1+i) = (c+id)+i(c-id) \\
		T^* &= T \\
		\NORM{T1}^2 &= \ABRACKET{T1, T1} = \ABRACKET{1+i, 1+i} = 2 \\
		\NORM{T} &= \sqrt{2} = \NORM{T^*} \\
		\NORM{TT^*} &= 2 \\
		TT^* &= 2I \\
		T_1 &= \frac{1}{2}\PAREN{(1+i)+(1+i)} = 1+i = T \\
		T_2 &= \frac{1}{2i}\PAREN{(1+i)-(1+i)} = 0 \\
	\end{align*}
\end{enumerate}
\end{document}